Proof of `add` function in Queue
The representation predicate for Queue segments was incorrect so I
ended up removing some auxiliary lemmas.  Some of these were not
useful to begin with in the context of Iris since it is much easier to
frame statements than it is in CFML.

rocq-osiris/stdlib/proofs/queue.v
@@ -36,6 +36,9 @@ Section boilerplate.
       types_to_repr := λ c n, {| content := c; next := n |};
       repr_id := λ '(c, n), eq_refl }.
 
+  Global Instance cons_inline : Inline "Cons" cell := {| inline_apply := Cons;
+                                                        inline_encode := λ _, eq_refl |}.
+
   Global Instance t_repr : RecordRepr t τ[Z; cell; cell] Mut :=
     { repr_to_types t := (t.(length), (t.(first), t.(last)));
       types_to_repr := λ l fst lst, {| length := l; first := fst; last := lst |};
@@ -43,100 +46,42 @@ Section boilerplate.
 
 End boilerplate.
 
-(* The [Cell], [Cell_Seg], and [Queue] resources.
-
-   I have tried to keep them faithful to the CFML definitions, but I have replaced the [IF] with a match.
-   Feel free to use [if decide (l = []) then ...] instead if you prefer. *)
+(* The [Cell], [Cell_Seg], and [Queue] resources.  *)
 
 Section queue_resources.
 
   Context `{!osirisGS Σ}.
 
-  Definition Cell `{Encode A} (v : A) (n c : cell) : iProp Σ :=
+  Definition Cell `{Encode A} (c n : cell) (v : A) : iProp Σ :=
     ∃ r,
       ⌜c = Cons r⌝ ∗ r ⤇ {| content := v; next := n |}.
 
-  Fixpoint Cell_Seg `{Encode A} (l : list A) (to from : cell) : iProp Σ :=
+  Fixpoint Cell_Seg `{Encode A} (from to : cell) (l : list A) : iProp Σ :=
     match l with
     | [] => ⌜to = from⌝
-    | x :: l' => ∃ n, Cell x n from ∗ Cell_Seg l' to n
+    | x :: l' => ∃ n, Cell from n x ∗ Cell_Seg n to l'
     end.
 
-  Definition Queue `{Encode A} (l : list A) (q : record) : iProp Σ :=
+  Definition Queue `{Encode A} (q : record) (l : list A) : iProp Σ :=
     ∃ (cf cl : cell),
       q ⤇ {| length := list_z.length l; first := cf; last := cl |} ∗
-      match l with
-      | [] => ⌜cf = Nil⌝ ∗ ⌜cl = Nil⌝
-      | x :: l' => Cell_Seg l' cl cf ∗ Cell_Seg [x] Nil cl
-      end.
+      if decide (l = nil) then
+        ⌜cf = Nil⌝ ∗ ⌜cl = Nil⌝
+      else
+        ∃ x l',
+          ⌜ l = l' ++ [x] ⌝ ∗
+          Cell_Seg cf cl l' ∗ Cell_Seg cl Nil [x].
 
-  Lemma Cell_Seg_nil `{Encode A} (to from : cell) :
-    Cell_Seg (@nil A) to from ∗-∗ ⌜to = from⌝.
-  Proof. auto. Qed.
-
-  Lemma Cell_Seg_Nil `{Encode A} :
-    ⊢ Cell_Seg (@nil A) Nil Nil.
-  Proof. auto. Qed.
-
-  Lemma Cell_Seg_cons `{Encode A} (x : A) (l : list A) (to from : cell) :
-    Cell_Seg (x :: l) to from -∗
-    ∃ n, Cell x n from ∗ Cell_Seg l to n.
-  Proof. auto. Qed.
-
-  Lemma Cell_Seg_Nil2 `{Encode A} (c : cell) (l : list A) :
-    Cell_Seg l c Nil -∗ ⌜l = []⌝ ∗ ⌜c = Nil⌝.
+  Lemma Cell_Seg_app A `{Encode A} r (x' : A) c cf l:
+      r ⤇ {| content := x'; next := c |} -∗
+      Cell_Seg cf (Cons r) l -∗
+      Cell_Seg cf c (l ++ [x']).
   Proof.
-    iIntros "HSeg".
-    destruct l as [|x l']; first auto.
-    iPoseProof (Cell_Seg_cons with "HSeg") as "(%n & HCell & _)".
-    iDestruct "HCell" as "(%r & %Hcontra & _)".
-    discriminate Hcontra.
-  Qed.
-
-  (* I have written [Queue_if] and [Queue_if_first] with a [match] and
-     an [if decide] respectively. Feel free to pick whichever style
-     you prefer. *)
-
-  Lemma Queue_if `{Encode A} (l : list A) (q : loc) :
-    Queue l q -∗
-    ∃ cf cl,
-      q ⤇ {| length := list_z.length l; first := cf; last := cl |} ∗
-      match cl with
-      | Nil => ⌜l = []⌝ ∗ ⌜cf = Nil⌝
-      | _ => ∃ x l', ⌜l = x :: l'⌝ ∗ Cell_Seg l' cl cf ∗ Cell_Seg [x] Nil cl
-      end.
-  Proof.
-    iIntros "(%cf & %cl & $ & Hl)".
-    destruct l as [|x l'].
-    { by iDestruct "Hl" as "(-> & ->)". }
-    simpl Cell_Seg.
-    iDestruct "Hl" as "(HSeg1 & (%n & HCell & <-))".
-    iDestruct "HCell" as "(%r & -> & Hr)".
-    by iFrame.
-  Qed.
-
-  Lemma Queue_if_first `{Encode A} (l : list A) (q : loc) :
-    Queue l q -∗
-    ∃ cf cl,
-      q ⤇ {| length := list_z.length l; first := cf; last := cl |} ∗
-      if decide (cf = Nil) then ⌜l = []⌝ ∗ ⌜cl = Nil⌝ else
-      ∃ x l', ⌜l = x :: l'⌝ ∗ Cell_Seg l' cl cf ∗ Cell_Seg [x] Nil cl.
-  Proof.
-    iIntros "(%cf & %cl & $ & Hl)".
-    destruct l as [|x l'].
-    { iDestruct "Hl" as "(-> & ->)". by case_decide. }
-    iDestruct "Hl" as "(HSeg1 & (%n & HCell & <-))".
-    iDestruct "HCell" as "(%r & -> & Hr)".
-    destruct l' as [|y l'']; simpl Cell_Seg.
-    { iDestruct "HSeg1" as "<-".
-      case_decide; first discriminate.
-      iExists x, []. iFrame.
-      equality. (* Osiris helper tactic to prove equalities. *) }
-    { iDestruct "HSeg1" as "(%n & HCell & HCell_Seg)".
-      iDestruct "HCell" as "(%r' & -> & Hr')".
-      case_decide; first discriminate.
-      iExists x, (y :: l''). iFrame.
-      equality. }
+    iIntros "C S".
+    iInduction l as [|h t Ih] forall (cf c).
+    - simpl. iDestruct "S" as "<-". by iFrame.
+    - simpl. iDestruct "S" as "(% & ? & S)".
+      iFrame. iApply ("Ih" with "[$] [$]").
   Qed.
 
 End queue_resources.
@@ -166,7 +111,7 @@ Section proofs.
      elements of that type. *)
 
   Definition create_spec (u : unit) (m : microvx) : iProp Σ :=
-    ∀ A (HencA : Encode A), EWP m {{ q, Queue (@nil A) q }}.
+    ∀ A (HencA : Encode A), EWP m {{ q, Queue q (@nil A) }}.
 
   Definition create := (EAnonFun __create).
 
@@ -192,6 +137,91 @@ Section proofs.
     simpl.
     iIntros (v) "(%l & %cf & %cl & Hv & -> & -> & ->)".
     unfold Queue. by iFrame.
+  Qed.
+
+  Definition add_spec {A} `{Encode A} (x : A) (_q : record) (m : microvx) : iProp Σ :=
+    ∀ (q : list A),
+      ▷ Queue _q q -∗
+      EWP m {{ (), Queue _q (q ++ [x]) }}.
+
+  Definition add := (EAnonFun __add).
+
+  Lemma imp_add η A `(Encode A) :
+    ⊢ EWP (eval η add) {{ f, □ iSpec τ[A;record] f add_spec }}.
+  Proof.
+    iApply imp_EAnon_pers. unfold add_spec.
+    iIntros "!> /= %x %q %l Hq".
+    iApply imp_please; iNext.
+    imp_let $! (λ (c : cell), Cell c Nil x).
+    { imp_record $! (cons (A:=A)). simpl.
+        iIntros "% (% & -> & (% & % & ? & -> & ->))".
+        by iFrame. }
+    iIntros "%c C".
+    iDestruct "Hq" as "(%cf & %cl& Ql & Q)".
+    imp_match cell with "[Ql]".
+    iIntros "(-> & Ql)". simpl.
+    destruct l as [|h t].
+    - iDestruct "Q" as "[-> ->]".
+      next_branch.
+      iApply (imp_ESeq with "[Ql]").
+      iApply (imp_record_update with "Ql").
+      { split; simpl; lia. }
+      { imp_path. }
+      { imp_int. }
+      { rewrite -encode_encode'.
+        simpl. iIntros "(%_ & -> & Ql)".
+        iApply (imp_ESeq with "[Ql]").
+        iApply (imp_record_update with "Ql");
+          try imp_path.
+        { split; simpl; lia. }
+        simpl. iIntros "(%_ & -> & Ql)".
+        iApply (imp_wand with "[-]").
+        iApply (imp_record_update with "Ql").
+        { split; simpl; lia. }
+        { imp_path. }
+        { set_postcondition
+            (λ c', Cell c' Nil x ∗ ⌜ c = c'⌝)%I.
+          imp_path.
+          by iFrame. }
+        simpl. iIntros "% (% & (? & <-) & ?)".
+        destruct v. iUnfold Queue.
+        iFrame. by iExists []. }
+    -
+      iDestruct "Q" as "(%x' & %l & -> & S & % & Cl & <-)".
+      iDestruct "Cl" as "(%r & -> & Cl)".
+      rewrite !(encode_encode' (A:=cell)).
+      rewrite <- (encode_encode' (A:=cell)).
+      next_branch.
+      next_branch.
+      iApply (imp_ESeq with "[Ql]").
+      {  set_postcondition (λ _, q ⤇ _)%I.
+         iApply (imp_record_update' with "[] [Ql]").
+      { split; simpl; lia. }
+      { imp_path. }
+      { imp_arith reading "Ql". iFrame "Ql".
+        imp_int. }
+      { simpl. iIntros "% (-> & $)".
+        iIntros "!>$". } }
+      simpl. iIntros "Ql".
+      iApply (imp_ESeq with "[Cl]").
+      iApply (imp_record_update with "Cl").
+      { split; simpl; lia. }
+      { imp_path. }
+      { imp_path. }
+      simpl. iIntros "(% & [-> Cl])".
+      iApply (imp_wand with "[Ql]").
+      iApply (imp_record_update with "Ql").
+      { split; simpl; lia. }
+      { imp_path. }
+      { imp_path. }
+      simpl. iIntros ([]) "(% & [-> Ql])".
+      iUnfold Queue.
+      list_z.length. iFrame "Ql".
+      rewrite decide_False.
+      2: { destruct l; discriminate. }
+      iExists x, (l ++ [x']).
+      iFrame. repeat iSplit; try done.
+      iApply (Cell_Seg_app with "[$] [$]").
   Qed.
 
 End proofs.
